$r(d,\theta) = E\Bigl[(d-E[d])^2]+(E[d]-\theta)^2\Bigr]$
$r(d,\theta)= E \Bigl[(d -E[d] + E[d] - \theta^2)\Bigr]$
$r(d,\theta) = E\Bigl[(d-E[d])^{2}+ (E[d] - \theta)^2 + 2(E[d] - \theta)(d-E[d])\Bigr]$
$r(d,\theta) = E\Bigl[ (d-E[d])^{2}\Bigr]+ E\Bigl[ (E[d] - \theta)^{2}\Bigr]+ 2E(E[d] - \theta)(d-E[d])$
$r(d,\theta) = E\Bigl[(d-E[d])^{2}\Bigr]+ (E[d])-\theta)^{2}+ 2(E[d]-\theta)E[d-E[d]]$
$r(d,\theta) = E[(d-E[d])^2] + (E[d]-\theta)^2$


- $Variance \longrightarrow E[(d-E[d])^2]$
- $Bias^2 \longrightarrow (E[d]-\theta)^2$

$r(d, \theta) = Var(d) + (b_{\theta}(d))^2$
